Weidenbach_Book/CDCL_Two_Watched_Literals_IsaSAT_CDCL.thy
@@ -21,8 +21,11 @@ subsection \<open>Code Generation\<close>
 
 subsubsection \<open>Types and Refinement Relations\<close>
 
-type_synonym trail_pol = \<open>(nat, nat) ann_lits \<times> bool option list \<times> nat list \<times> nat\<close>
-type_synonym trail_pol_assn = \<open>(uint32 \<times> nat option) list \<times> bool option array \<times> uint32 array \<times> uint32\<close>
+type_synonym trail_pol =
+   \<open>nat literal list \<times> bool option list \<times> nat list \<times> nat option list \<times> nat\<close>
+
+type_synonym trail_pol_assn =
+   \<open>uint32 list \<times> bool option array \<times> uint32 array \<times> nat option array \<times> uint32\<close>
 
 type_synonym twl_st_wll_trail =
   \<open>trail_pol_assn \<times> clauses_wl \<times> nat \<times> conflict_option_assn \<times>
@@ -38,11 +41,20 @@ definition polarity_atm where
 definition get_level_atm where
   \<open>get_level_atm M L = get_level M (Pos L)\<close>
 
+
 context isasat_input_ops
 begin
 
+definition ann_lits_split_reasons where
+  \<open>ann_lits_split_reasons = {((M, reasons), M'). M = map lit_of M' \<and> 
+    (\<forall>L \<in> set M'. is_proped L \<longrightarrow> reasons ! (atm_of (lit_of L)) = Some (mark_of L)) \<and> 
+    (\<forall>L \<in> set M'. is_decided L \<longrightarrow> reasons ! (atm_of (lit_of L)) = None) \<and>
+    (\<forall>L \<in># \<L>\<^sub>a\<^sub>l\<^sub>l. atm_of L < length reasons)
+  }\<close>
+
 definition trail_pol :: \<open>(trail_pol \<times> (nat, nat) ann_lits) set\<close> where
-  \<open>trail_pol = {((M', xs, lvls, k), M). M = M' \<and> no_dup M \<and>
+  \<open>trail_pol = {((M', xs, lvls, reasons, k), M). ((M', reasons), M) \<in> ann_lits_split_reasons \<and>
+    no_dup M \<and>
     (\<forall>L \<in># \<L>\<^sub>a\<^sub>l\<^sub>l. atm_of L < length xs \<and> xs ! (atm_of L) = polarity_atm M (atm_of L)) \<and>
     (\<forall>L \<in># \<L>\<^sub>a\<^sub>l\<^sub>l. atm_of L < length lvls \<and> lvls ! (atm_of L) = get_level M L) \<and>
     k = count_decided M \<and>
@@ -51,8 +63,10 @@ definition trail_pol :: \<open>(trail_pol \<times> (nat, nat) ann_lits) set\<clo
 end
 
 abbreviation trail_pol_assn :: \<open>trail_pol \<Rightarrow> trail_pol_assn \<Rightarrow> assn\<close> where
-  \<open>trail_pol_assn \<equiv> pair_nat_ann_lits_assn *assn array_assn (option_assn bool_assn) *assn
-      array_assn uint32_nat_assn *assn uint32_nat_assn\<close>
+  \<open>trail_pol_assn \<equiv> 
+      list_assn unat_lit_assn *assn array_assn (option_assn bool_assn) *assn
+      array_assn uint32_nat_assn *assn
+      array_assn (option_assn nat_assn) *assn uint32_nat_assn\<close>
 
 abbreviation phase_saver_conc where
   \<open>phase_saver_conc \<equiv> array_assn bool_assn\<close>
@@ -421,7 +435,8 @@ lemmas get_level_code_get_level_code[sepref_fr_rules] =
    get_level_code.refine[of \<A>\<^sub>i\<^sub>n, OF isasat_input_bounded_axioms]
 
 definition (in -) count_decided_pol where
-  \<open>count_decided_pol = (\<lambda>(_, _, _, k). k)\<close>
+  \<open>count_decided_pol = (\<lambda>(_, _, _, _, k). k)\<close>
+
 lemma count_decided_trail_ref:
   \<open>(RETURN o count_decided_pol, RETURN o count_decided) \<in> trail_pol \<rightarrow>\<^sub>f \<langle>nat_rel\<rangle>nres_rel\<close>
   by (intro frefI nres_relI) (auto simp: trail_pol_def count_decided_pol_def)
@@ -1568,17 +1583,24 @@ definition cons_trail_Propagated :: \<open>nat literal \<Rightarrow> nat \<Right
   \<open>cons_trail_Propagated L C M' = Propagated L C # M'\<close>
 
 definition cons_trail_Propagated_tr :: \<open>nat literal \<Rightarrow> nat \<Rightarrow> trail_pol \<Rightarrow> trail_pol\<close> where
-  \<open>cons_trail_Propagated_tr = (\<lambda>L C (M', xs, lvls, k).
-     (Propagated L C # M', xs[atm_of L := Some (is_pos L)],
-      lvls[atm_of L := k], k))\<close>
+  \<open>cons_trail_Propagated_tr = (\<lambda>L C (M', xs, lvls, reasons, k).
+     (L # M', xs[atm_of L := Some (is_pos L)],
+      lvls[atm_of L := k], reasons[atm_of L:= Some C], k))\<close>
 
+lemma in_list_pos_neg_notD: \<open>Pos (atm_of (lit_of La)) \<notin> lits_of_l bc \<Longrightarrow>
+       Neg (atm_of (lit_of La)) \<notin> lits_of_l bc \<Longrightarrow>
+       La \<in> set bc \<Longrightarrow> False\<close>
+  by (metis Neg_atm_of_iff Pos_atm_of_iff lits_of_def rev_image_eqI)
+  
 
 lemma cons_trail_Propagated_tr:
   \<open>(uncurry2 (RETURN ooo cons_trail_Propagated_tr), uncurry2 (RETURN ooo cons_trail_Propagated)) \<in>
   [\<lambda>((L, C), M). undefined_lit M L \<and> L \<in> snd ` D\<^sub>0]\<^sub>f Id \<times>\<^sub>f nat_rel \<times>\<^sub>f trail_pol \<rightarrow> \<langle>trail_pol\<rangle>nres_rel\<close>
   by (intro frefI nres_relI, rename_tac x y, case_tac \<open>fst (fst x)\<close>)
-    (auto simp: trail_pol_def polarity_atm_def cons_trail_Propagated_def uminus_lit_swap
-        cons_trail_Propagated_tr_def Decided_Propagated_in_iff_in_lits_of_l nth_list_update')
+    (fastforce simp: trail_pol_def polarity_atm_def cons_trail_Propagated_def uminus_lit_swap
+        cons_trail_Propagated_tr_def Decided_Propagated_in_iff_in_lits_of_l nth_list_update'
+        ann_lits_split_reasons_def atms_of_\<L>\<^sub>a\<^sub>l\<^sub>l_\<A>\<^sub>i\<^sub>n 
+        dest!: in_list_pos_neg_notD dest: pos_lit_in_atms_of neg_lit_in_atms_of)+
 
 lemma undefined_lit_count_decided_uint_max:
   assumes
@@ -1618,7 +1640,8 @@ qed
 
 sepref_thm cons_trail_Propagated_tr_code
   is \<open>uncurry2 (RETURN ooo cons_trail_Propagated_tr)\<close>
-  :: \<open>[\<lambda>((L, C), (M, xs, lvls, k)). atm_of L < length xs \<and> atm_of L < length lvls]\<^sub>a
+  :: \<open>[\<lambda>((L, C), (M, xs, lvls, reasons, k)). atm_of L < length xs \<and> atm_of L < length lvls \<and>
+     atm_of L < length reasons]\<^sub>a
        unat_lit_assn\<^sup>k *\<^sub>a nat_assn\<^sup>k *\<^sub>a trail_pol_assn\<^sup>d \<rightarrow> trail_pol_assn\<close>
   unfolding cons_trail_Propagated_tr_def cons_trail_Propagated_tr_def
   supply [[goals_limit = 1]]
@@ -1642,7 +1665,8 @@ proof -
   have H: \<open>(uncurry2 cons_trail_Propagated_tr_code, uncurry2 (RETURN \<circ>\<circ>\<circ> cons_trail_Propagated))
     \<in> [comp_PRE (Id \<times>\<^sub>f nat_rel \<times>\<^sub>f trail_pol)
      (\<lambda>((L, C), M). undefined_lit M L \<and> L \<in> snd ` D\<^sub>0)
-     (\<lambda>_ ((L, C), (M, xs, lvls, k)). atm_of L < length xs \<and> atm_of L < length lvls)
+     (\<lambda>_ ((L, C), (M, xs, lvls, reasons, k)). atm_of L < length xs \<and> atm_of L < length lvls \<and>
+        atm_of L < length reasons)
      (\<lambda>_. True)]\<^sub>a hrp_comp
                      (unat_lit_assn\<^sup>k *\<^sub>a nat_assn\<^sup>k *\<^sub>a trail_pol_assn\<^sup>d)
                      (Id \<times>\<^sub>f nat_rel \<times>\<^sub>f
@@ -1651,7 +1675,7 @@ proof -
     using hfref_compI_PRE_aux[OF cons_trail_Propagated_tr_code.refine cons_trail_Propagated_tr,
         OF isasat_input_bounded_axioms] .
   have pre: \<open>?pre' = ?pre\<close>
-    by (auto simp: comp_PRE_def trail_pol_def trail_pol_def intro!: ext)
+    by (auto simp: comp_PRE_def trail_pol_def trail_pol_def ann_lits_split_reasons_def intro!: ext)
   have im: \<open>?im' = ?im\<close>
     unfolding prod_hrp_comp hrp_comp_dest hrp_comp_keep
     by (auto simp: hrp_comp_def hr_comp_def)
@@ -2937,16 +2961,78 @@ lemma is_decided_hd_trail_wl_heur_is_decided_hd_trail_wl:
 lemma get_trail_wl_heur_def: \<open>get_trail_wl_heur = (\<lambda>(M, S). M)\<close>
   by (intro ext, rename_tac S, case_tac S) auto
 
-definition (in -) hd_trail_code :: \<open>trail_pol_assn \<Rightarrow> uint32 \<times> nat option\<close> where
-  \<open>hd_trail_code = (\<lambda>(M, _). hd M)\<close>
+definition (in -) hd_trail_pol :: \<open>trail_pol \<Rightarrow> (nat literal \<times> nat option) nres\<close> where
+  \<open>hd_trail_pol = (\<lambda>(M, xs, lvls, reasons, k). do { 
+      ASSERT(atm_of (hd M) < length reasons);
+      RETURN (hd M, reasons ! (atm_of (hd M)))})\<close>
 
-lemma hd_trail_code_hd[sepref_fr_rules]:
-  \<open>(return o hd_trail_code, RETURN o op_list_hd) \<in> [\<lambda>M. M \<noteq> []]\<^sub>a trail_assn\<^sup>k \<rightarrow> pair_nat_ann_lit_assn\<close>
-  unfolding hd_trail_code_def op_list_hd_def
-  apply sepref_to_hoare
-  apply (case_tac x; case_tac xi; case_tac \<open>fst (xi)\<close>)
-  apply (sep_auto simp:  trail_pol_def hr_comp_def)+
+
+sepref_definition (in -)hd_trail_code
+  is \<open>hd_trail_pol\<close>
+  :: \<open>[\<lambda>(M, xs, lvls, reasons, k). M \<noteq> []]\<^sub>a
+       trail_pol_assn\<^sup>k \<rightarrow> unat_lit_assn *assn (option_assn nat_assn)\<close>
+  unfolding hd_trail_pol_def nth_u_def[symmetric]
+  supply [[goals_limit = 1]]
+  by sepref
+
+lemmas cons_trail_Propagated_tr_code[sepref_fr_rules] =
+  cons_trail_Propagated_tr_code.refine[OF isasat_input_bounded_axioms]
+
+lemma (in -)is_propedE: \<open>is_proped L \<Longrightarrow> (\<And>K C. L = Propagated K C \<Longrightarrow> P) \<Longrightarrow> P\<close>
+  by (cases L) auto
+
+lemma hd_trail_pol_op_list_hd:
+  \<open>(hd_trail_pol, RETURN o op_list_hd) \<in> [\<lambda>M. M \<noteq> []]\<^sub>f trail_pol \<rightarrow> 
+     \<langle>{((L, C), L'). (C = None \<longrightarrow> L' = Decided L) \<and> (C \<noteq> None \<longrightarrow> L' = Propagated L (the C))}\<rangle> nres_rel\<close>
+  by (intro frefI nres_relI)
+     (auto simp: trail_pol_def hd_trail_pol_def ann_lits_split_reasons_def hd_map
+      elim!: neq_NilE is_decided_ex_Decided not_is_decidedE 
+      simp: is_decided_no_proped_iff[symmetric])
+
+lemma (in -) nat_ann_lit_rel_alt_def: \<open>nat_ann_lit_rel = (unat_lit_rel \<times>\<^sub>r \<langle>nat_rel\<rangle> option_rel) O
+     {((L, C), L').
+      (C = None \<longrightarrow> L' = Decided L) \<and>
+      (C \<noteq> None \<longrightarrow> L' = Propagated L (the C))}\<close>
+  apply (rule; rule)
+  subgoal for x
+    by (cases x; cases \<open>fst x\<close>)
+      (auto simp: nat_ann_lit_rel_def pure_def ann_lit_of_pair_alt_def hr_comp_def
+        ex_assn_pair_split unat_lit_rel_def uint32_nat_rel_def br_def nat_lit_rel_def
+        Collect_eq_comp lit_of_natP_def case_prod_beta relcomp.simps
+        split: if_splits)
+  subgoal for x
+    by (cases x; cases \<open>fst x\<close>)
+      (auto simp: nat_ann_lit_rel_def pure_def ann_lit_of_pair_alt_def hr_comp_def
+        ex_assn_pair_split unat_lit_rel_def uint32_nat_rel_def br_def nat_lit_rel_def
+        Collect_eq_comp lit_of_natP_def case_prod_beta relcomp.simps
+        split: if_splits)
   done
+   
+lemma hd_trail_code_hd[sepref_fr_rules]:
+  \<open>(hd_trail_code, RETURN o op_list_hd) \<in> [\<lambda>M. M \<noteq> []]\<^sub>a trail_assn\<^sup>k \<rightarrow> pair_nat_ann_lit_assn\<close>
+     (is \<open>?c \<in> [?pre]\<^sub>a ?im \<rightarrow> ?f\<close>)
+proof -
+  have H: \<open>?c \<in>  [comp_PRE trail_pol (\<lambda>M. M \<noteq> [])
+       (\<lambda>_ (M, xs, lvls, reasons, k). M \<noteq> [])
+       (\<lambda>_. True)]\<^sub>a hrp_comp (trail_pol_assn\<^sup>k)
+                      trail_pol \<rightarrow> hr_comp
+  (unat_lit_assn *assn option_assn nat_assn)
+  {((L, C), L').
+   (C = None \<longrightarrow> L' = Decided L) \<and>
+   (C \<noteq> None \<longrightarrow> L' = Propagated L (the C))}\<close>
+    (is \<open>_ \<in> [?pre']\<^sub>a ?im' \<rightarrow> ?f'\<close>)
+    using hfref_compI_PRE_aux[OF hd_trail_code.refine hd_trail_pol_op_list_hd] .
+  have pre: \<open>?pre' = ?pre\<close>
+    by (auto simp: comp_PRE_def trail_pol_def trail_pol_def ann_lits_split_reasons_def intro!: ext)
+  have im: \<open>?im' = ?im\<close>
+    unfolding prod_hrp_comp hrp_comp_dest hrp_comp_keep
+    by (auto simp: hrp_comp_def hr_comp_def)
+  have f: \<open>?f' = ?f\<close>
+    unfolding  nat_ann_lit_rel_alt_def hr_comp_pure[symmetric] prod_assn_pure_conv[symmetric]
+      option_assn_pure_conv[symmetric] ..
+  show ?thesis
+    using H unfolding im pre f .
+qed
 
 sepref_thm is_decided_hd_trail_wl_code
   is \<open>RETURN o is_decided_hd_trail_wl_heur\<close>
@@ -3235,20 +3321,20 @@ lemma tl_state_wl_heur_alt_def:
   by (auto simp: tl_state_wl_heur_def Let_def)
 
 definition (in isasat_input_ops) tl_trailt_tr :: \<open>trail_pol \<Rightarrow> trail_pol\<close> where
-  \<open>tl_trailt_tr = (\<lambda>(M', xs, lvls, k). (tl M', xs[atm_of (lit_of (hd M')) := None], lvls[atm_of (lit_of (hd M')) := 0],
-    if is_decided (hd M') then k-1 else k))\<close>
+  \<open>tl_trailt_tr = (\<lambda>(M', xs, lvls, reasons, k). (tl M', xs[atm_of (hd M') := None], 
+    lvls[atm_of (hd M') := zero_uint32_nat],
+    reasons, if reasons ! atm_of (hd M') = None then k-one_uint32_nat else k))\<close>
 
 sepref_thm tl_trail_tr_code
   is \<open>RETURN o tl_trailt_tr\<close>
-  :: \<open>[\<lambda>(M, xs, lvls, k). M \<noteq> [] \<and> atm_of (lit_of (hd M)) < length xs  \<and> atm_of (lit_of (hd M)) < length lvls \<and>
-    (is_decided (hd M) \<longrightarrow> k \<ge> 1)]\<^sub>a
+  :: \<open>[\<lambda>(M, xs, lvls, reason, k). M \<noteq> [] \<and> atm_of (hd M) < length xs  \<and> atm_of (hd M) < length lvls \<and>
+      atm_of (hd M) < length reason \<and>
+    (reason ! atm_of (hd M) = None \<longrightarrow> k \<ge> 1)]\<^sub>a
         trail_pol_assn\<^sup>d \<rightarrow> trail_pol_assn\<close>
   supply if_splits[split] option.splits[split]
   unfolding tl_trailt_tr_def
-  apply (rewrite at \<open>_ - 1\<close> fast_minus_def[symmetric])
+  apply (rewrite at \<open>_ - one_uint32_nat\<close> fast_minus_def[symmetric])
   supply [[goals_limit = 1]]
-  supply uint32_nat_assn_one[sepref_fr_rules]
-  supply uint32_nat_assn_zero[sepref_fr_rules]
   by sepref
 
 concrete_definition (in -) tl_trail_tr_code
@@ -3259,6 +3345,10 @@ prepare_code_thms (in -) tl_trail_tr_code_def
 
 lemmas tl_trail_tr_coded_refine[sepref_fr_rules] =
    tl_trail_tr_code.refine[of \<A>\<^sub>i\<^sub>n, OF isasat_input_bounded_nempty_axioms]
+
+lemma (in isasat_input_ops) ann_lits_split_reasons_map_lit_of:
+  \<open>((M, reasons), M') \<in> ann_lits_split_reasons \<Longrightarrow> M = map lit_of M'\<close>
+  by (auto simp: ann_lits_split_reasons_def)
 
 lemma tl_trail_tr:
   \<open>((RETURN o tl_trailt_tr), (RETURN o tl)) \<in>
@@ -3271,20 +3361,24 @@ proof -
       unfolding trail_pol_def comp_def RETURN_refine_iff trail_pol_def
       apply clarify
       apply (intro conjI; clarify?; (intro conjI)?)
-      subgoal by (auto simp: trail_pol_def polarity_atm_def tl_trailt_tr_def)
+      subgoal by (auto simp: trail_pol_def polarity_atm_def tl_trailt_tr_def 
+            ann_lits_split_reasons_def)
       subgoal by (auto simp: trail_pol_def polarity_atm_def tl_trailt_tr_def)
       subgoal by (auto simp: polarity_atm_def tl_trailt_tr_def)
       subgoal
         by (cases \<open>lit_of L\<close>)
-            (auto simp: polarity_atm_def tl_trailt_tr_def Decided_Propagated_in_iff_in_lits_of_l)
+          (auto simp: polarity_atm_def tl_trailt_tr_def Decided_Propagated_in_iff_in_lits_of_l 
+            dest!: ann_lits_split_reasons_map_lit_of)
       subgoal
         by (auto simp: polarity_atm_def tl_trailt_tr_def
            atm_of_eq_atm_of get_level_cons_if)
       subgoal
         by (auto simp: polarity_atm_def tl_trailt_tr_def
-           atm_of_eq_atm_of get_level_cons_if)
+           atm_of_eq_atm_of get_level_cons_if
+            dest!: ann_lits_split_reasons_map_lit_of)
       subgoal
-        by (auto simp: tl_trailt_tr_def in_\<L>\<^sub>a\<^sub>l\<^sub>l_atm_of_in_atms_of_iff
+        by (cases \<open>L\<close>)
+          (auto simp: tl_trailt_tr_def in_\<L>\<^sub>a\<^sub>l\<^sub>l_atm_of_in_atms_of_iff ann_lits_split_reasons_def
             dest: no_dup_consistentD vmtf_unset_vmtf_tl)
       subgoal
         by (auto simp: tl_trailt_tr_def)
@@ -3295,28 +3389,38 @@ qed
 lemma tl_trail_tr_code_op_list_tl[sepref_fr_rules]:
   \<open>(tl_trail_tr_code, (RETURN o op_list_tl)) \<in>
     [\<lambda>M. M \<noteq> []]\<^sub>a trail_assn\<^sup>d \<rightarrow> trail_assn\<close>
-    (is \<open>_ \<in> [?pre]\<^sub>a ?im \<rightarrow> ?f\<close>)
+    (is \<open>_?c\<in> [?pre]\<^sub>a ?im \<rightarrow> ?f\<close>)
 proof -
-  have [dest]: \<open>((a, aa, ab, b), x) \<in> trail_pol \<Longrightarrow> x = a\<close> for a aa ab b x
-    by (auto simp: trail_pol_def)
+  have [dest]: \<open>((a, aa, ab, r, b), x) \<in> trail_pol \<Longrightarrow> a = map lit_of x\<close> for a aa ab b x r
+    by (auto simp: trail_pol_def ann_lits_split_reasons_def)
   have [simp]: \<open>x \<noteq> [] \<Longrightarrow> is_decided (hd x) \<Longrightarrow> Suc 0 \<le> count_decided x\<close> for x
     by (cases x) auto
-  have H: \<open>(tl_trail_tr_code, RETURN \<circ> tl)
-      \<in> [comp_PRE trail_pol (\<lambda>M. M \<noteq> [])
-            (\<lambda>_ (M, xs, lvls, k). M \<noteq> [] \<and> atm_of (lit_of (hd M)) < length xs \<and>
-             atm_of (lit_of (hd M)) < length lvls \<and> (is_decided (hd M) \<longrightarrow> 1 \<le> k))
-            (\<lambda>_. True)]\<^sub>a
-         hrp_comp (trail_pol_assn\<^sup>d) trail_pol \<rightarrow> hr_comp trail_pol_assn trail_pol\<close>
+  have H: \<open>?c
+      \<in>  [comp_PRE trail_pol (\<lambda>M. M \<noteq> [])
+     (\<lambda>_ (M, xs, lvls, reason, k).
+         M \<noteq> [] \<and>
+         atm_of (hd M) < length xs \<and>
+         atm_of (hd M) < length lvls \<and>
+         atm_of (hd M) < length reason \<and>
+         (reason ! atm_of (hd M) = None \<longrightarrow> 1 \<le> k))
+     (\<lambda>_. True)]\<^sub>a hrp_comp (trail_pol_assn\<^sup>d)
+                    trail_pol \<rightarrow> hr_comp trail_pol_assn trail_pol\<close>
     (is \<open>_ \<in> [?pre']\<^sub>a ?im' \<rightarrow> ?f'\<close>)
-    using hfref_compI_PRE_aux[OF tl_trail_tr_code.refine tl_trail_tr, OF isasat_input_bounded_nempty_axioms] .
-  have pre: \<open>?pre' = ?pre\<close>
-    by (auto simp: comp_PRE_def trail_pol_def phase_saving_def
-        in_\<L>\<^sub>a\<^sub>l\<^sub>l_atm_of_in_atms_of_iff vmtf_def intro!: ext)
+    using hfref_compI_PRE_aux[OF tl_trail_tr_code.refine tl_trail_tr, OF isasat_input_bounded_nempty_axioms] 
+    unfolding op_list_tl_def
+    .
+  have pre: \<open>?pre x \<Longrightarrow> ?pre' x\<close> for x
+    apply (cases x; cases \<open>hd x\<close>)
+    by (auto simp: comp_PRE_def trail_pol_def phase_saving_def ann_lits_split_reasons_def
+         vmtf_def intro!: ext)
   have im: \<open>?im' = ?im\<close>
     unfolding prod_hrp_comp hrp_comp_dest hrp_comp_keep
     by (auto simp: hrp_comp_def hr_comp_def)
   show ?thesis
-    using H unfolding im pre by simp
+    apply (rule hfref_weaken_pre[OF ])
+     defer
+    using H unfolding im apply assumption
+    using pre ..
 qed
 
 fun get_vmtf_heur :: \<open>twl_st_wl_heur \<Rightarrow> _\<close> where
@@ -4352,13 +4456,13 @@ definition (in -) lit_of_hd_trail_st :: \<open>'v twl_st_wl \<Rightarrow> 'v lit
   \<open> lit_of_hd_trail_st S = lit_of (hd (get_trail_wl S))\<close>
 
 definition lit_of_hd_trail_st_heur :: \<open>twl_st_wl_heur_trail_ref \<Rightarrow> nat literal\<close> where
-  \<open>lit_of_hd_trail_st_heur = (\<lambda>((M, _), _). lit_of (hd M))\<close>
+  \<open>lit_of_hd_trail_st_heur = (\<lambda>((M, _), _). hd M)\<close>
 
 lemma lit_of_hd_trail_st_heur_lit_of_hd_trail_st:
    \<open>(RETURN o lit_of_hd_trail_st_heur, RETURN o lit_of_hd_trail_st) \<in>
        [\<lambda>S. get_trail_wl S \<noteq> []]\<^sub>f twl_st_heur_pol \<rightarrow> \<langle>Id\<rangle>nres_rel\<close>
   by (auto simp: lit_of_hd_trail_st_def twl_st_heur_pol_def trail_pol_def
-       lit_of_hd_trail_st_heur_def
+       lit_of_hd_trail_st_heur_def ann_lits_split_reasons_def hd_map
       intro!: frefI nres_relI)
 
 sepref_thm lit_of_hd_trail_st_code
@@ -4391,7 +4495,8 @@ proof -
     using hfref_compI_PRE_aux[OF lit_of_hd_trail_st_code_refine_code
     lit_of_hd_trail_st_heur_lit_of_hd_trail_st] .
   have pre: \<open>?pre' x\<close> if \<open>?pre x\<close> for x
-    using that by (auto simp: comp_PRE_def twl_st_heur_pol_def trail_pol_def)
+    using that by (auto simp: comp_PRE_def twl_st_heur_pol_def trail_pol_def
+        ann_lits_split_reasons_def)
   have im: \<open>?im' = ?im\<close>
     unfolding prod_hrp_comp hrp_comp_dest hrp_comp_keep twl_st_heur_assn_assn ..
   have f: \<open>?f' = ?f\<close>
@@ -5228,12 +5333,13 @@ definition (in -) lit_of_hd_trail where
   \<open>lit_of_hd_trail M = lit_of (hd M)\<close>
 
 definition (in -) lit_of_hd_trail_pol where
-  \<open>lit_of_hd_trail_pol = (\<lambda>(M, _). lit_of (hd M))\<close>
+  \<open>lit_of_hd_trail_pol = (\<lambda>(M, _). hd M)\<close>
 
 lemma lit_of_hd_trail_pol_lit_of_hd_trail:
    \<open>(RETURN o lit_of_hd_trail_pol, RETURN o lit_of_hd_trail) \<in>
          [\<lambda>S. S \<noteq> []]\<^sub>f trail_pol \<rightarrow> \<langle>Id\<rangle>nres_rel\<close>
-   by (auto simp: lit_of_hd_trail_def trail_pol_def lit_of_hd_trail_pol_def
+  by (auto simp: lit_of_hd_trail_def trail_pol_def lit_of_hd_trail_pol_def
+     ann_lits_split_reasons_def hd_map
       intro!: frefI nres_relI)
 
 sepref_definition (in -) lit_of_hd_trail_code
@@ -5255,7 +5361,8 @@ proof -
     using hfref_compI_PRE_aux[OF lit_of_hd_trail_code.refine
       lit_of_hd_trail_pol_lit_of_hd_trail] .
   have pre: \<open>?pre' x\<close> if \<open>?pre x\<close> for x
-    using that by (auto simp: comp_PRE_def twl_st_heur_pol_def trail_pol_def)
+    using that by (auto simp: comp_PRE_def twl_st_heur_pol_def trail_pol_def
+       ann_lits_split_reasons_def)
   have im: \<open>?im' = ?im\<close>
     unfolding prod_hrp_comp hrp_comp_dest hrp_comp_keep twl_st_heur_assn_assn ..
   have f: \<open>?f' = ?f\<close>
@@ -8204,9 +8311,9 @@ proof -
     for M xs lvls k M' L
   proof -
     have
-       \<open>M = M'\<close> and
+       \<open>M' = map lit_of M\<close> and
        \<open>\<forall>L\<in>#\<L>\<^sub>a\<^sub>l\<^sub>l. atm_of L < length xs \<and> xs ! atm_of L = polarity_atm M (atm_of L)\<close>
-      using tr unfolding trail_pol_def by fast+
+      using tr unfolding trail_pol_def ann_lits_split_reasons_def by fast+
     then have L: \<open>L < length xs\<close> and xsL: \<open>xs ! L = polarity_atm M L\<close>
       using L_N by force+
     show ?length
@@ -8520,26 +8627,27 @@ definition cons_trail_Decided :: \<open>nat literal \<Rightarrow> (nat, nat) ann
   \<open>cons_trail_Decided L M' = Decided L # M'\<close>
 
 definition cons_trail_Decided_tr :: \<open>nat literal \<Rightarrow> trail_pol \<Rightarrow> trail_pol\<close> where
-  \<open>cons_trail_Decided_tr = (\<lambda>L (M', xs, lvls, k).
-     (Decided L # M', xs[atm_of L := Some (is_pos L)],
-      lvls[atm_of L := k+1], k+1))\<close>
+  \<open>cons_trail_Decided_tr = (\<lambda>L (M', xs, lvls, reasons, k).
+     (L # M', xs[atm_of L := Some (is_pos L)],
+      lvls[atm_of L := k+1], reasons[atm_of L := None], k+1))\<close>
 
 lemma cons_trail_Decided_tr:
   \<open>(uncurry (RETURN oo cons_trail_Decided_tr), uncurry (RETURN oo cons_trail_Decided)) \<in>
   [\<lambda>(L, M). undefined_lit M L \<and> L \<in> snd ` D\<^sub>0]\<^sub>f Id \<times>\<^sub>f trail_pol \<rightarrow> \<langle>trail_pol\<rangle>nres_rel\<close>
   by (intro frefI nres_relI, rename_tac x y, case_tac \<open>fst x\<close>)
-     (auto simp: trail_pol_def polarity_atm_def cons_trail_Decided_def uminus_lit_swap
-        trail_pol_def cons_trail_Decided_tr_def Decided_Propagated_in_iff_in_lits_of_l
-        cons_trail_Decided_tr_def nth_list_update'
-      intro: vmtf_consD)
+    (fastforce simp: trail_pol_def polarity_atm_def cons_trail_Decided_def uminus_lit_swap
+        Decided_Propagated_in_iff_in_lits_of_l
+        cons_trail_Decided_tr_def nth_list_update' ann_lits_split_reasons_def
+      intro: vmtf_consD dest!: in_list_pos_neg_notD)+
 
 sepref_thm cons_trail_Decided_tr_code
   is \<open>uncurry (RETURN oo cons_trail_Decided_tr)\<close>
-  :: \<open>[\<lambda>(L, (M, xs, lvls, k)). undefined_lit M L \<and> atm_of L < length xs \<and> atm_of L < length lvls \<and>
-     (\<forall>L\<in>set M. lit_of L \<in># \<L>\<^sub>a\<^sub>l\<^sub>l) \<and> no_dup M \<and> L \<in> snd ` D\<^sub>0 \<and> k = count_decided M]\<^sub>a
+  :: \<open>[\<lambda>(L, (M, xs, lvls, reason, k)). atm_of L < length xs \<and> atm_of L < length lvls \<and>
+     atm_of L < length reason \<and> L \<in> snd ` D\<^sub>0 \<and>
+      Suc k \<le> uint_max]\<^sub>a
        unat_lit_assn\<^sup>k *\<^sub>a trail_pol_assn\<^sup>d \<rightarrow> trail_pol_assn\<close>
   unfolding cons_trail_Decided_tr_def cons_trail_Decided_tr_def one_uint32_nat_def[symmetric]
-  supply [[goals_limit = 1]] undefined_lit_count_decided_uint_max[dest!]
+  supply [[goals_limit = 1]]
   by sepref
 
 concrete_definition (in -) cons_trail_Decided_tr_code
@@ -8557,24 +8665,22 @@ lemma cons_trail_Decided_tr_code_cons_trail_Decided_tr[sepref_fr_rules]:
     trail_assn\<close>
     (is \<open>?c \<in> [?pre]\<^sub>a ?im \<rightarrow> ?f\<close>)
 proof -
-  have H: \<open>?c \<in> [comp_PRE (nat_lit_lit_rel \<times>\<^sub>f trail_pol)
+  have H: \<open>?c \<in>  [comp_PRE (nat_lit_lit_rel \<times>\<^sub>f trail_pol)
      (\<lambda>(L, M). undefined_lit M L \<and> L \<in> snd ` D\<^sub>0)
-     (\<lambda>_ (L, M, xs, lvls, k).
-         undefined_lit M L \<and>
+     (\<lambda>_ (L, M, xs, lvls, reason, k).
          atm_of L < length xs \<and>
          atm_of L < length lvls \<and>
-         (\<forall>L\<in>set M. lit_of L \<in># \<L>\<^sub>a\<^sub>l\<^sub>l) \<and>
-         no_dup M \<and> L \<in> snd ` D\<^sub>0 \<and> k = count_decided M)
-     (\<lambda>_. True)]\<^sub>a hrp_comp
-                     (unat_lit_assn\<^sup>k *\<^sub>a trail_pol_assn\<^sup>d)
-                     (nat_lit_lit_rel \<times>\<^sub>f
-                      trail_pol) \<rightarrow> hr_comp trail_pol_assn
-         trail_pol\<close>
+         atm_of L < length reason \<and> L \<in> snd ` D\<^sub>0 \<and> Suc k \<le> uint_max)
+     (\<lambda>_. True)]\<^sub>a hrp_comp (unat_lit_assn\<^sup>k *\<^sub>a trail_pol_assn\<^sup>d)
+                    (nat_lit_lit_rel \<times>\<^sub>f
+                     trail_pol) \<rightarrow> hr_comp trail_pol_assn trail_pol\<close>
     (is \<open>_ \<in> [?pre']\<^sub>a ?im' \<rightarrow> ?f'\<close>)
     using hfref_compI_PRE_aux[OF cons_trail_Decided_tr_code.refine cons_trail_Decided_tr,
         OF isasat_input_bounded_nempty_axioms] .
+  thm  undefined_lit_count_decided_uint_max[dest!]
   have pre: \<open>?pre' = ?pre\<close>
-    by (auto simp: comp_PRE_def trail_pol_def trail_pol_def image_image intro!: ext)
+    by (auto simp: comp_PRE_def trail_pol_def image_image ann_lits_split_reasons_def intro!: ext
+        intro!: undefined_lit_count_decided_uint_max)
   have im: \<open>?im' = ?im\<close>
     unfolding prod_hrp_comp hrp_comp_dest hrp_comp_keep
     by (auto simp: hrp_comp_def hr_comp_def)
